new-semantics/coq/events/EnvSemantics.v
@@ -100,6 +100,16 @@ Proof.
   try eqb2eq loc; clarify; eauto.
 Qed.
 
+Lemma read_env_subst {var loc lang} `{Eq var} `{Eq loc} (σ : nv var loc lang) :
+  forall ℓ ν w x (READ : read_env σ x = Env_wvl w),
+    read_env (subst_loc_nv ν ℓ σ) x = Env_wvl (subst_loc_wvl ν ℓ w).
+Proof.
+  induction σ; ii; ss;
+  des_ifs; ss;
+  des_ifs; eqb2eq var; clarify;
+  try eqb2eq loc; clarify; eauto.
+Qed.
+
 Lemma read_env_floc {var loc lang} `{Eq var} `{Eq loc} (σ : nv var loc lang) :
   forall w ℓ x (READ : read_env σ x = Env_wvl w) (IN : In ℓ (floc_wvl w)),
     In ℓ (floc_nv σ).
@@ -110,20 +120,13 @@ Proof.
   rewrite in_app_iff; eauto.
 Qed.
 
-Lemma eval_floc_dec {var loc} `{Eq var} `{Name loc} t (σ : nv var loc (@val var)) v (EVAL : eval σ t v) :
+Lemma eval_floc_dec {var loc} `{Eq var} `{Eq loc} t (σ : nv var loc (@val var)) v (EVAL : eval σ t v) :
   forall ℓ (IN : In ℓ (floc_vl v)), In ℓ (floc_nv σ).
 Proof.
   induction EVAL; ii; ss; eauto.
   - eapply read_env_floc; eauto.
-  - gensym_tac (floc_vl v) ν.
-    assert (subst_intro_vl _ _ _ v) as RR by eapply subst_intro.
-    rewrite RR in IN; eauto.
-    assert (floc_subst_wvl_vl _ _ _ (open_loc_vl 0 ν v)) as HINT by eapply floc_subst_wvl.
-    apply HINT in IN.
-    des; ss.
-    apply open_floc in IN0. des; clarify.
-    eapply read_env_floc; eauto.
-    eapply read_env_floc; eauto.
+  - eapply open_wvl_floc in IN.
+    ss; des; eapply read_env_floc; eauto.
   - apply IHEVAL3 in IN.
     rewrite in_app_iff in IN; des; auto.
   - rewrite in_app_iff in IN; des; auto.
@@ -154,24 +157,6 @@ Proof.
     rrw; eauto.
 Qed.
 
-Lemma eval_subst {var loc} `{Eq var} `{Name loc} t (σ : nv var loc (@val var)) v (EVAL : eval σ t v) :
-  forall ℓ' ν (FRESH : ~ In ν (floc_nv σ)),
-    eval (subst_loc_nv ν ℓ' σ) t (subst_loc_vl ν ℓ' v).
-Proof.
-  ii. pose proof (eval_map t σ v EVAL (swap id ν ℓ')) as HINT.
-  assert (swap_is_subst_nv _ _ _ σ) as RR by eapply swap_is_subst.
-  assert (swap_is_subst_vl _ _ _ v) as RR' by eapply swap_is_subst.
-  replace ν with (id ν) by reflexivity.
-  replace ℓ' with (id ℓ') by reflexivity.
-  replace σ with (map_nv id σ) by (eapply map_id_is_id).
-  replace v with (map_vl id v) by (eapply map_id_is_id).
-  rewrite <- RR. rewrite <- RR'.
-  apply HINT.
-  ii; unfold swap, id in fEQ; des_ifs; repeat eqb2eq loc; clarify.
-  all:try solve [ii; ss].
-  red. intros IN. eapply eval_floc_dec in EVAL; eauto.
-Qed.
-
 Lemma read_env_wvl {var loc lang} `{Eq var} `{Eq loc} (σ : nv var loc lang) x :
   forall r w ℓ (READ : read_env σ x = r),
     read_env (subst_wvl_nv w ℓ σ) x =
@@ -188,7 +173,80 @@ Proof.
   exploit IHσ; eauto; ss; repeat rw; eauto.
 Qed.
 
-Lemma eval_subst_wvl {var loc} `{Eq var} `{Name loc} t (σ : nv var loc (@val var)) v (EVAL : eval σ t v) :
+Lemma eval_map_subst_loc {var loc} `{Eq var} `{Name loc} t (σ : nv var loc (@val var)) v (EVAL : eval σ t v) :
+  forall φ (INJ : oto φ) ν ℓ',
+    eval (subst_loc_nv ν ℓ' (map_nv φ σ)) t (subst_loc_vl ν ℓ' (map_vl φ v)).
+Proof.
+  induction EVAL; ii; ss;
+  try solve [econstructor; eauto].
+  - econstructor 1.
+    eapply read_env_map with (φ := φ) in READ. ss.
+    exploit (read_env_subst _ _ _ _ x); eauto.
+  - assert (map_open_wvl_vl _ _ _ v) by (eapply map_open_wvl; auto).
+    rw. s.
+    assert (open_wvl_subst_loc_vl _ _ _ (map_vl φ v)) by (eapply open_wvl_subst_loc; auto).
+    rw; eauto.
+    econstructor 2.
+    eapply read_env_map with (φ := φ) in READ. ss.
+    exploit (read_env_subst _ _ _ _ x); eauto.
+  - specialize (IHEVAL2 φ INJ ν ℓ').
+    assert (map_close_vl _ _ _ v1) as RR by (eapply map_close; auto).
+    rewrite RR in *; auto. clear RR.
+    gensym_tac (ℓ' :: φ ℓ :: ν :: floc_nv (map_nv φ σ)) ℓ''. clear Heqℓ''.
+    assert (~ In ℓ'' (floc_vl (map_vl φ v1))) as HINT.
+    { intro. apply eval_map with (φ := φ) in EVAL1; auto.
+      eapply eval_floc_dec in EVAL1; eauto. ss. des; ss. }
+    replace 
+      (close_vl 0 (φ ℓ) (map_vl φ v1)) with
+      (close_vl 0 ℓ'' (subst_loc_vl ℓ'' (φ ℓ) (map_vl φ v1))) in *.
+    replace 
+      (subst_loc_vl ν ℓ' (close_vl 0 ℓ'' (subst_loc_vl ℓ'' (φ ℓ) (map_vl φ v1)))) with
+      (close_vl 0 ℓ'' (subst_loc_vl ν ℓ' (subst_loc_vl ℓ'' (φ ℓ) (map_vl φ v1)))) in *.
+    constructor; auto.
+    { intro IN. eapply floc_subst_loc in IN. des; auto. }
+    { set (compose loc (swap id ℓ'' (φ ℓ)) φ) as φ'.
+      replace (map_nv φ σ) with (map_nv φ' σ).
+      replace (subst_loc_vl ℓ'' (φ ℓ) (map_vl φ v1)) with (map_vl φ' v1).
+      exploit (IHEVAL1 φ' _ ν).
+      subst φ'. unfold compose, swap, id.
+      ii; ss; des_ifs;
+      repeat match goal with
+      | _ => eqb2eq loc
+      | H : φ _ = φ _ |- _ => apply INJ in H
+      | _ => clarify
+      end.
+      instantiate (1 := ℓ').
+      replace (eqb ℓ' (φ' ℓ)) with false.
+      replace (φ' ℓ) with ℓ''. auto.
+      1, 2: subst φ'; unfold compose, swap, id; s; des_ifs; eqb2eq loc; clarify.
+      symmetry. apply eqb_neq. auto.
+      { assert (swap_is_subst_vl _ _ _ (map_vl φ v1)) as RR by eapply swap_is_subst.
+        specialize (RR id).
+        exploit RR; eauto. unfold oto. auto.
+        instantiate (1 := φ ℓ).
+        replace (map_vl id (map_vl φ v1)) with (map_vl φ v1) by (symmetry; eapply map_id_is_id).
+        unfold id at 2. unfold id at 2.
+        intro. rrw.
+        subst φ'. symmetry. eapply map_compose. }
+      { eapply map_ext.
+        ii. subst φ'. unfold compose, swap, id.
+        des_ifs; eqb2eq loc; clarify.
+        eapply floc_map in DOM; eauto. contradict.
+        exploit INJ; eauto. ii; clarify. } }
+    { eapply subst_loc_close; auto. }
+    { eapply subst_loc_close_eq; auto. }
+Qed.
+
+Lemma eval_subst_loc {var loc} `{Eq var} `{Name loc} t (σ : nv var loc (@val var)) v (EVAL : eval σ t v) :
+  forall ν ℓ', eval (subst_loc_nv ν ℓ' σ) t (subst_loc_vl ν ℓ' v).
+Proof.
+  intros.
+  replace σ with (map_nv id σ) by apply map_id_is_id.
+  replace v with (map_vl id v) by apply map_id_is_id.
+  eapply eval_map_subst_loc; try intro; auto.
+Qed.
+
+Lemma eval_map_subst_wvl {var loc} `{Eq var} `{Name loc} t (σ : nv var loc (@val var)) v (EVAL : eval σ t v) :
   forall φ (INJ : oto φ)
     u (U : wvalue u) ℓ',
     eval (subst_wvl_nv u ℓ' (map_nv φ σ)) t (subst_wvl_vl u ℓ' (map_vl φ v)).
@@ -252,3 +310,14 @@ Proof.
     { eapply subst_wvl_close; auto. }
     { eapply subst_loc_close_eq; auto. }
 Qed.
+
+Lemma eval_subst_wvl {var loc} `{Eq var} `{Name loc} t (σ : nv var loc (@val var)) v (EVAL : eval σ t v) :
+  forall u (U : wvalue u) ℓ',
+    eval (subst_wvl_nv u ℓ' σ) t (subst_wvl_vl u ℓ' v).
+Proof.
+  intros.
+  replace σ with (map_nv id σ) by apply map_id_is_id.
+  replace v with (map_vl id v) by apply map_id_is_id.
+  eapply eval_map_subst_wvl; try intro; auto.
+Qed.
+
