new-semantics/coq/events/LinkFacts.v
@@ -1,0 +1,423 @@
+From Basics Require Import Basics.
+From With_events Require Import Defs.
+From With_events Require Import Syntax.
+From With_events Require Import SubstFacts.
+From With_events Require Import EnvSemantics.
+From With_events Require Import LinkDefs.
+
+Section LinkFacts.
+  Variable var : Type.
+  Variable loc : Type.
+
+  #[local] Coercion vl_ev : vnt >-> vl.
+  #[local] Coercion vl_exp : nv >-> vl.
+  #[local] Coercion wvl_v : vl >-> wvl.
+
+  Ltac link_lc_tac := 
+    repeat match goal with
+    | _ => solve [auto]
+    | H : wvalue (_ _) |- _ => inv H
+    | H : env (_ _) |- _ => inv H
+    | H : value (_ _) |- _ => inv H
+    | H : event (_ _) |- _ => inv H
+    | _ => instantiate (1 := [])
+    end.
+
+  Lemma link_lc `{Eq loc} `{Eq var} (σ0 : nv var loc _) (w : wvl var loc _) :
+    forall w' (LINK : σ0 ⋊ w ∋ w'), wvalue w.
+  Proof.
+    ii. induction LINK;
+    repeat econstructor; des;
+    link_lc_tac; ii.
+    all: match goal with
+    | RR : _ = open_loc_vl 0 ?ν ?v |- value (open_loc_vl 0 ?ℓ ?v) =>
+      assert (value (open_loc_vl 0 ν v)) by (rewrite <- RR; constructor; auto);
+      replace (open_loc_vl 0 ℓ v) with (subst_loc_vl ℓ ν (open_loc_vl 0 ν v))
+    end.
+    all: try match goal with
+    | V : value ?v |- value (subst_loc_vl _ _ ?v) =>
+      assert (subst_loc_lc_vl _ _ _ v V) by eapply subst_loc_lc; auto
+    | |- context [subst_loc_vl ?ℓ ?ν (open_loc_vl 0 ?ν ?v)] =>
+      assert (open_loc_subst_loc_vl _ _ _ v) by eapply open_loc_subst_loc;
+      rw; rewrite eqb_refl;
+      f_equal; eapply subst_loc_fresh; auto
+    end.
+  Qed.
+
+  Ltac linked_lc_tac := 
+    repeat match goal with
+    | _ => solve [auto]
+    | H : wvalue (_ _) |- _ => inv H
+    | H : env (_ _) |- _ => inv H
+    | H : value (_ _) |- _ => inv H
+    | H : event (_ _) |- _ => inv H
+    | _ => instantiate (1 := [])
+    end.
+
+  Lemma linked_lc_wvl `{Name loc} `{Eq var}
+    (σ0 : nv var loc _) (Σ0 : env σ0) (w : wvl var loc _) :
+    forall w' (LINK : σ0 ⋊ w ∋ w'), wvalue w'.
+  Proof.
+    ii. induction LINK;
+    repeat econstructor; des;
+    linked_lc_tac; ii.
+    - eapply read_env_lc in READ; auto.
+      destruct w; inv READ; ss.
+      assert (subst_intro_vl _ _ _ v) by eapply subst_intro.
+      gensym_tac (L ++ floc_vl v) ℓ.
+      rw; eauto.
+      eapply subst_wvl_lc; eauto.
+      econstructor; eauto.
+    - eapply eval_lc in EVAL; eauto.
+      repeat econstructor; eauto.
+    - assert (close_open_loc_eq_vl _ _ _ v') by eapply close_open_loc_eq.
+      rw.
+      assert (open_loc_lc_vl _ _ _ v' VAL) by (eapply open_loc_lc; eauto).
+      rw.
+      eapply subst_loc_lc; auto.
+  Qed.
+
+  Lemma map_unroll {lang} `{Eq loc} φ (w : wvl var loc lang) :
+    unroll (map_wvl φ w) = map_vl φ (unroll w).
+  Proof.
+    destruct w; ss.
+    assert (map_open_wvl_vl _ _ _ v) by eapply map_open_wvl.
+    rw; ss.
+  Qed.
+
+  Lemma subst_loc_unroll {lang} `{Eq loc}
+    ℓ ν (w : wvl var loc lang) :
+    unroll (subst_loc_wvl ν ℓ w) = subst_loc_vl ν ℓ (unroll w).
+  Proof.
+    destruct w; ss.
+    match goal with
+    | |- context [subst_loc_vl _ _ (open_wvl_vl _ _ ?v)] =>
+      assert (open_wvl_subst_loc_vl _ _ _ v)
+        by (eapply open_wvl_subst_loc; eauto);
+      rw; ss
+    end.
+  Qed.
+
+  Lemma subst_wvl_unroll {lang} `{Name loc}
+    ℓ (u w : wvl var loc lang) (U : wvalue u) :
+    unroll (subst_wvl_wvl u ℓ w) = subst_wvl_vl u ℓ (unroll w).
+  Proof.
+    destruct w; ss.
+    match goal with
+    | |- context [subst_wvl_vl _ _ (open_wvl_vl _ _ ?v)] =>
+      assert (open_wvl_subst_wvl_vl _ _ _ v)
+        by (eapply open_wvl_subst_wvl; eauto);
+      rw; ss
+    end.
+  Qed.
+
+  Lemma unroll_floc {lang} ℓ (w : wvl var loc lang) :
+    In ℓ (floc_wvl w) <-> In ℓ (floc_vl (unroll w)).
+  Proof.
+    split; intro IN; destruct w; ss.
+    - eapply open_wvl_inc_floc. auto.
+    - eapply open_wvl_floc in IN. ss; des; auto.
+  Qed.
+
+  Lemma link_floc_dec `{Eq loc} `{Eq var}
+    (σ0 : nv var loc _) (w w' : wvl var loc _) (LINK : σ0 ⋊ w ∋ w') :
+    forall ℓ (IN : In ℓ (floc_wvl w')), In ℓ (floc_nv σ0) \/ In ℓ (floc_wvl w).
+  Proof.
+    induction LINK; ii; ss;
+    repeat match goal with
+    | _ => solve [auto]
+    | _ => rewrite in_app_iff
+    | EVAL : context [eval] |- _ => eapply eval_floc_dec in EVAL; eauto; ss
+    | IN : In _ (floc_vl (unroll _)) |- _ => rewrite <- unroll_floc in IN
+    | IN : In _ (?a ++ ?b) |- _ => rewrite in_app_iff in IN
+    | IN : _ \/ _ |- _ => destruct IN as [IN | IN]
+    | IN : In _ ?l, Hl : forall x, In x ?l -> _ |- _ => specialize (Hl _ IN)
+    end.
+    - eapply IHLINK.
+      eapply read_env_floc; eauto.
+    - eapply close_floc in IN.
+      des; exploit IHLINK; eauto; intro IN'; des; auto.
+      eapply open_floc in IN'; des; clarify; auto.
+  Qed.
+
+  Lemma link_map `{Name loc} `{Eq var}
+    (σ0 : nv var loc _) (w w' : wvl var loc _) (LINK : σ0 ⋊ w ∋ w') :
+    forall φ (INJ : oto φ),
+      map_nv φ σ0 ⋊ map_wvl φ w ∋ map_wvl φ w'.
+  Proof.
+    induction LINK; ii; ss;
+    try solve [econstructor; eauto].
+    - rewrite <- map_unroll.
+      apply read_env_map with (φ := φ) in READ.
+      econstructor; eauto.
+    - specialize (IHLINK1 φ INJ).
+      specialize (IHLINK2 φ INJ).
+      eapply link_CallEval; eauto.
+      eapply eval_map with (φ := φ) in EVAL; eauto.
+    - assert (map_close_vl _ _ _ v') by (eapply map_close; eauto).
+      rw; eauto.
+      econstructor; eauto;
+      match goal with
+      | |- ~ In _ _ =>
+        intro IN; eapply map_floc in IN; eauto
+      | _ =>
+        specialize (IHLINK φ INJ);
+        assert (map_open_loc_vl _ _ _ v) as RR by (eapply map_open_loc; eauto);
+        rewrite RR in *; auto
+      end.
+  Qed.
+
+  Lemma link_map_subst_loc `{Name loc} `{Eq var}
+    (σ0 : nv var loc _) (w w' : wvl var loc _) (LINK : σ0 ⋊ w ∋ w') :
+    forall φ (INJ : oto φ) ν ℓ',
+      subst_loc_nv ν ℓ' (map_nv φ σ0) ⋊
+      subst_loc_wvl ν ℓ' (map_wvl φ w) ∋
+      subst_loc_wvl ν ℓ' (map_wvl φ w').
+  Proof.
+    induction LINK; ii; ss;
+    try solve [econstructor; eauto].
+    - rewrite <- map_unroll.
+      rewrite <- subst_loc_unroll.
+      apply read_env_map with (φ := φ) in READ.
+      econstructor; eauto.
+      apply read_env_subst; auto.
+    - specialize (IHLINK1 φ INJ ν ℓ').
+      specialize (IHLINK2 φ INJ ν ℓ').
+      eapply link_CallEval; eauto.
+      eapply eval_map_subst_loc with (ν := ν) (ℓ' := ℓ') in EVAL; eauto.
+      assumption.
+    - des_goal; eqb2eq loc; clarify;
+      econstructor; eauto.
+    - assert (map_close_vl _ _ _ v') as RR by (eapply map_close; auto).
+      rewrite RR; eauto. clear RR.
+      gensym_tac (ℓ' :: φ ℓ :: ν :: floc_nv (map_nv φ σ0) ++ floc_vl (map_vl φ v)) ℓ''.
+      clear Heqℓ''.
+      assert (~ In ℓ'' (floc_vl (map_vl φ v'))) as HINT.
+      { intro. apply link_map with (φ := φ) in LINK; auto; ss.
+        eapply link_floc_dec in LINK; eauto. des; ss.
+        assert (map_open_loc_vl _ _ _ v) as RR by (eapply map_open_loc; eauto).
+        rewrite RR in *. eapply open_floc in LINK. des; ss; clarify. }
+      replace
+        (close_vl 0 (φ ℓ) (map_vl φ v')) with
+        (close_vl 0 ℓ'' (subst_loc_vl ℓ'' (φ ℓ) (map_vl φ v'))) by
+      (eapply subst_loc_close_eq; auto).
+      replace 
+        (subst_loc_vl ν ℓ' (close_vl 0 ℓ'' (subst_loc_vl ℓ'' (φ ℓ) (map_vl φ v')))) with
+        (close_vl 0 ℓ'' (subst_loc_vl ν ℓ' (subst_loc_vl ℓ'' (φ ℓ) (map_vl φ v')))) by
+      (eapply subst_loc_close; auto).
+      econstructor; eauto.
+      { intro IN. eapply floc_subst_loc in IN. des; auto. }
+      { intro IN. eapply floc_subst_loc in IN. des; auto. }
+      { set (compose loc (swap id ℓ'' (φ ℓ)) φ) as φ'.
+        exploit (IHLINK φ' _ ν).
+        subst φ'. unfold compose, swap, id.
+        ii; ss; des_ifs;
+        repeat match goal with
+        | _ => eqb2eq loc
+        | H : φ _ = φ _ |- _ => apply INJ in H
+        | _ => clarify
+        end.
+        instantiate (1 := ℓ').
+        assert (map_open_loc_vl _ _ _ v) as RR by (eapply map_open_loc; eauto).
+        rw. clear RR. replace (φ' ℓ) with ℓ''.
+        assert (open_loc_subst_loc_vl _ _ _ (map_vl φ' v)) as RR by (eapply open_loc_subst_loc; eauto).
+        rw. clear RR. replace (eqb ℓ' ℓ'') with false.
+        replace (map_nv φ σ0) with (map_nv φ' σ0).
+        replace (map_vl φ v) with (map_vl φ' v).
+        replace (subst_loc_vl ℓ'' (φ ℓ) (map_vl φ v')) with (map_vl φ' v').
+        auto.
+        { assert (swap_is_subst_vl _ _ _ (map_vl φ v')) as RR by eapply swap_is_subst.
+          specialize (RR id).
+          exploit RR; eauto. unfold oto. auto.
+          instantiate (1 := φ ℓ).
+          replace (map_vl id (map_vl φ v')) with (map_vl φ v') by (symmetry; eapply map_id_is_id).
+          unfold id at 2. unfold id at 2.
+          intro. rrw.
+          subst φ'. symmetry. eapply map_compose. }
+        { eapply map_ext.
+          ii. subst φ'. unfold compose, swap, id.
+          des_ifs; eqb2eq loc; clarify.
+          eapply floc_map in DOM; eauto. contradict.
+          exploit INJ; eauto. ii; clarify. }
+        { eapply map_ext.
+          ii. subst φ'. unfold compose, swap, id.
+          des_ifs; eqb2eq loc; clarify.
+          eapply floc_map in DOM; eauto. contradict.
+          exploit INJ; eauto. ii; clarify. }
+        { symmetry. eqb2eq loc. auto. }
+        { subst φ'. unfold compose, swap, id.
+          rewrite eqb_refl. des_goal; eqb2eq loc; clarify. } }
+  Qed.
+
+  Lemma link_subst_loc `{Name loc} `{Eq var}
+    (σ0 : nv var loc _) (w w' : wvl var loc _) (LINK : σ0 ⋊ w ∋ w') :
+    forall ν ℓ',
+      subst_loc_nv ν ℓ' σ0 ⋊ subst_loc_wvl ν ℓ' w ∋ subst_loc_wvl ν ℓ' w'.
+  Proof.
+    intros.
+    replace σ0 with (map_nv id σ0) by apply map_id_is_id.
+    replace w with (map_wvl id w) by apply map_id_is_id.
+    replace w' with (map_wvl id w') by apply map_id_is_id.
+    eapply link_map_subst_loc; try intro; auto.
+  Qed.
+
+  Lemma link_map_subst_wvl `{Name loc} `{Eq var}
+    (σ0 : nv var loc _) (Σ0 : env σ0) (w w' : wvl var loc _) (LINK : σ0 ⋊ w ∋ w') :
+    forall φ (INJ : oto φ) u u' (LINKu : map_nv φ σ0 ⋊ u ∋ u') ℓ' (nIN : ~ In ℓ' (floc_nv (map_nv φ σ0))),
+      map_nv φ σ0 ⋊
+      subst_wvl_wvl u ℓ' (map_wvl φ w) ∋
+      subst_wvl_wvl u' ℓ' (map_wvl φ w').
+  Proof.
+    do 4 intros.
+    eapply link_lc in LINKu as U.
+    eapply linked_lc_wvl in LINKu as U';
+    try eapply map_lc; eauto.
+    revert_until LINK.
+    induction LINK; ii; ss;
+    try solve [econstructor; eauto].
+    - assert (subst_wvl_fresh_nv _ _ _ (map_nv φ σ0)) by (eapply subst_wvl_fresh; eauto).
+      rw; eauto. econstructor; eauto.
+    - rewrite <- map_unroll.
+      rewrite <- subst_wvl_unroll; auto.
+      apply read_env_map with (φ := φ) in READ.
+      econstructor; eauto.
+      erewrite read_env_wvl; eauto; ss.
+    - specialize (IHLINK1 φ INJ u u' LINKu ℓ' nIN U U').
+      specialize (IHLINK2 φ INJ u u' LINKu ℓ' nIN U U').
+      eapply link_CallEval; eauto.
+      eapply eval_map_subst_wvl with (u := u') (ℓ' := ℓ') in EVAL; eauto.
+      assumption.
+    - des_goal; eqb2eq loc; clarify;
+      try solve [econstructor; eauto].
+    - assert (map_close_vl _ _ _ v') as RR by (eapply map_close; auto).
+      rewrite RR; eauto. clear RR.
+      gensym_tac (ℓ' :: φ ℓ :: floc_wvl u ++ floc_nv (map_nv φ σ0) ++ floc_vl (map_vl φ v)) ℓ''.
+      clear Heqℓ''.
+      assert (~ In ℓ'' (floc_vl (map_vl φ v'))) as HINT.
+      { intro. apply link_map with (φ := φ) in LINK; auto; ss.
+        eapply link_floc_dec in LINK; eauto. des; ss.
+        assert (map_open_loc_vl _ _ _ v) as RR by (eapply map_open_loc; eauto).
+        rewrite RR in *. eapply open_floc in LINK. des; ss; clarify. }
+      assert (~ In ℓ'' (floc_wvl u')) as HINT'.
+      { intro. eapply link_floc_dec in LINKu; eauto. des; ss. }
+      replace
+        (close_vl 0 (φ ℓ) (map_vl φ v')) with
+        (close_vl 0 ℓ'' (subst_loc_vl ℓ'' (φ ℓ) (map_vl φ v'))) by
+      (eapply subst_loc_close_eq; auto).
+      replace 
+        (subst_wvl_vl u' ℓ' (close_vl 0 ℓ'' (subst_loc_vl ℓ'' (φ ℓ) (map_vl φ v')))) with
+        (close_vl 0 ℓ'' (subst_wvl_vl u' ℓ' (subst_loc_vl ℓ'' (φ ℓ) (map_vl φ v')))) by
+      (eapply subst_wvl_close; auto).
+      econstructor; eauto.
+      { intro IN. eapply floc_subst_wvl in IN. des; auto. }
+      { set (compose loc (swap id ℓ'' (φ ℓ)) φ) as φ'.
+        assert (map_nv φ σ0 = map_nv φ' σ0) as HINT''.
+        { eapply map_ext.
+          ii. subst φ'. unfold compose, swap, id.
+          des_ifs; eqb2eq loc; clarify.
+          eapply floc_map in DOM; eauto. contradict.
+          exploit INJ; eauto. ii; clarify. }
+        exploit (IHLINK φ' _ u u'); eauto; try instantiate (1 := ℓ').
+        subst φ'. unfold compose, swap, id.
+        ii; ss; des_ifs;
+        repeat match goal with
+        | _ => eqb2eq loc
+        | H : φ _ = φ _ |- _ => apply INJ in H
+        | _ => clarify
+        end.
+        all: rrw; auto.
+        assert (map_open_loc_vl _ _ _ v) as RR by (eapply map_open_loc; eauto).
+        rw. clear RR. replace (φ' ℓ) with ℓ''.
+        assert (open_loc_subst_wvl_vl _ _ _ (map_vl φ' v)) as RR by (eapply open_loc_subst_wvl; eauto).
+        rw; eauto. clear RR.
+        replace (map_vl φ v) with (map_vl φ' v).
+        replace (subst_loc_vl ℓ'' (φ ℓ) (map_vl φ v')) with (map_vl φ' v').
+        auto.
+        { assert (swap_is_subst_vl _ _ _ (map_vl φ v')) as RR by eapply swap_is_subst.
+          specialize (RR id).
+          exploit RR; eauto. unfold oto. auto.
+          instantiate (1 := φ ℓ).
+          replace (map_vl id (map_vl φ v')) with (map_vl φ v') by (symmetry; eapply map_id_is_id).
+          unfold id at 2. unfold id at 2.
+          intro. rrw.
+          subst φ'. symmetry. eapply map_compose. }
+        { eapply map_ext.
+          ii. subst φ'. unfold compose, swap, id.
+          des_ifs; eqb2eq loc; clarify.
+          eapply floc_map in DOM; eauto. contradict.
+          exploit INJ; eauto. ii; clarify. }
+        { subst φ'. unfold compose, swap, id.
+          rewrite eqb_refl. des_goal; eqb2eq loc; clarify. } }
+  Qed.
+
+  Lemma link_subst_wvl `{Name loc} `{Eq var}
+    (σ0 : nv var loc _) (Σ0 : env σ0) (w w' : wvl var loc _) (LINK : σ0 ⋊ w ∋ w') :
+    forall u u' (LINKu : σ0 ⋊ u ∋ u') ℓ' (nIN : ~ In ℓ' (floc_nv σ0)),
+      σ0 ⋊ subst_wvl_wvl u ℓ' w ∋ subst_wvl_wvl u' ℓ' w'.
+  Proof.
+    intros.
+    assert (map_nv id σ0 = σ0) as RR by apply map_id_is_id.
+    rewrite <- RR.
+    replace w with (map_wvl id w) by apply map_id_is_id.
+    replace w' with (map_wvl id w') by apply map_id_is_id.
+    eapply link_map_subst_wvl; try rewrite RR; try intro; eauto.
+  Qed.
+
+  Lemma link_vl `{Eq loc} `{Eq var} (σ0 : nv var loc _) (v : vl var loc _) w (LINK : σ0 ⋊ v ∋ w) :
+    match w with
+    | wvl_v _ => True
+    | _ => False
+    end.
+  Proof.
+    inv LINK; clarify.
+  Qed.
+
+  Lemma link_read `{Name loc} `{Eq var} (σ0 : nv var loc _) (Σ0 : env σ0) :
+    forall (σ : nv var loc _) x (w w' σ' : wvl var loc _)
+      (LINK : σ0 ⋊ σ ∋ σ')
+      (READ : read_env σ x = Env_wvl w),
+    match σ' with
+    | wvl_v (vl_exp σ') =>
+      read_env σ' x = Env_wvl w' -> (σ0 ⋊ unroll w ∋ unroll w')
+    | _ => False
+    end.
+  Proof.
+    induction σ; ii; ss; repeat des_goal; inv LINK; clarify.
+    - intros. repeat econstructor; eauto.
+    - intros. ss; clarify. econstructor.
+      instantiate (1 := nv_ev E').
+      eapply link_holeEvent; auto. ss.
+    - ss; des_ifs; eqb2eq var.
+      ii. exploit IHσ; eauto.
+    - ss; des_ifs; eqb2eq var; clarify.
+      + ii; clarify;
+        match goal with
+        | |- context [unroll ?w] =>
+          destruct w; ss
+        end.
+        * eapply link_vl in LINKw as HINT.
+          destruct w'; clarify.
+        * inv LINKw; ss.
+          assert (subst_intro_vl _ _ _ (close_vl 0 ℓ v')) by eapply subst_intro.
+          rw. instantiate (1 := ℓ).
+          assert (close_open_loc_eq_vl _ _ _ v') by eapply close_open_loc_eq.
+          rw.
+          assert (subst_id_vl _ _ _ (open_loc_vl 0 ℓ v')) by eapply subst_id.
+          rw.
+          assert (subst_intro_vl _ _ _ v) by eapply subst_intro.
+          rw. instantiate (1 := ℓ).
+          repeat match goal with
+          | |- context [wvl_v (subst_wvl_vl ?a ?b ?c)] =>
+            replace (wvl_v (subst_wvl_vl a b c)) with
+              (subst_wvl_wvl a b (wvl_v c)) by reflexivity
+          end.
+          eapply link_subst_wvl; eauto.
+          eapply linked_lc_wvl in LINKv as V'; eauto. inv V'.
+          assert (open_loc_lc_vl _ _ _ v' VAL) by (eapply open_loc_lc; eauto).
+          rw. auto.
+          econstructor; eauto.
+          auto.
+          intro IN. eapply close_floc in IN. des; clarify.
+      + exploit IHσ; eauto.
+  Qed.
+End LinkFacts.
